define varrayp using mk_selector_vprop

pulse/ulib/experimental/Steel.Array0.fst
@@ -2,77 +2,51 @@ module Steel.Array0
 
 /// Definition of the selector and its vprop
 
-let pts_to'
+let pts_to' // necessary because of the selector return type
   (#elt: Type0) (a: array elt)
   (p: P.perm)
   (s: Seq.lseq elt (length a))
-: Tot slprop
-= hp_of (pts_to a p s)
+: Tot vprop
+= pts_to a p s
 
-let varrayp_hp a p =
-  Steel.Memory.h_exists (pts_to' a p)
-
-let varrayp_sel' 
-  (#elt: Type) (a: array elt) (p: P.perm)
-: Tot (selector' (Seq.lseq elt (length a)) (varrayp_hp a p))
-= fun m -> id_elim_exists (pts_to' a p) m
-
-module M = Steel.Memory
-
-let varrayp_sel_depends_only_on
-  (#elt: Type)
-  (a: array elt)
+let pts_to'_inj
+  (#elt: Type0) (a: array elt)
   (p: P.perm)
-  (m0: Steel.Memory.hmem (varrayp_hp a p))
-  (m1: mem { disjoint m0 m1 })
-: Lemma
-  (
-    varrayp_sel' a p m0 == varrayp_sel' a p (M.join m0 m1)
-  )
-  [SMTPat (varrayp_sel' a p (M.join m0 m1))]
-= pts_to_inj a p (varrayp_sel' a p m0) p (varrayp_sel' a p (M.join m0 m1)) (M.join m0 m1)
+: Tot (interp_hp_of_injective (pts_to' a p))
+= fun x1 x2 m -> pts_to_inj a p x1 p x2 m
 
-let varrayp_sel_depends_only_on_core
-  (#elt: Type)
-  (a: array elt)
-  (p: P.perm)
-  (m0: Steel.Memory.hmem (varrayp_hp a p))
-: Lemma
-  (
-    varrayp_sel' a p m0 == varrayp_sel' a p (core_mem m0)
-  )
-  [SMTPat (varrayp_sel' a p (core_mem m0))]
-= pts_to_inj a p (varrayp_sel' a p m0) p (varrayp_sel' a p (core_mem m0)) m0
+// _hp and _sel are declared in the interface so that
+// [@@__steel_reduce__] gives users the selector return type by
+// normalization. Alternatively, we could define varrayp directly with
+// mk_selector_vprop in the interface, but to strengthen the selector
+// return type, we would then need to declare pts_to' and pts_to'_inj
+// in the interface.
 
-let varrayp_sel a p = varrayp_sel' a p
+let varrayp_hp a p = mk_selector_vprop_hp (pts_to' a p)
+let varrayp_sel a p = mk_selector_vprop_sel _ (pts_to'_inj a p)
 
 let intro_varrayp
   a p s
 =
   pts_to_length a p _;
-  change_slprop_rel
-    (pts_to a p _)
+  change_equal_slprop
+    (pts_to a p s)
+    (pts_to' a p s);
+  mk_selector_vprop_intro _ (pts_to'_inj a p);
+  change_equal_slprop
+    (mk_selector_vprop _ _)
     (varrayp a p)
-    (fun _ s' -> s `Seq.equal` s')
-    (fun m ->
-      intro_h_exists s (pts_to' a p) m;
-      let s' = varrayp_sel' a p m in
-      pts_to_inj a p s p s' m
-    )
 
 let elim_varrayp
   #_ #elt a p
 =
-  let s0 = gget (varrayp a p) in
-  let refinement (s: Seq.lseq elt (length a)) : Tot prop = s == Ghost.reveal s0 in
-  let s1 : Ghost.erased (Seq.seq elt) = Ghost.reveal s0 in
-  intro_vrefine (varrayp a p) refinement;
-  rewrite_slprop
-    (varrayp a p `vrefine` refinement)
-    (pts_to a p s1)
-    (fun m ->
-      interp_vrefine_hp (varrayp a p) refinement m
-      // injectivity is not needed, because the return value of the
-      // selector is exactly the witness of exists_
-    );
-  s1
+  change_equal_slprop
+    (varrayp a p)
+    (mk_selector_vprop _ (pts_to'_inj a p));
+  let res0 = mk_selector_vprop_elim _ (pts_to'_inj a p) in
+  // the following is necessary because the selector return type changed
+  let res : Ghost.erased (Seq.seq elt) = Ghost.hide (Ghost.reveal res0) in
+  change_equal_slprop
+    (pts_to' a p res0)
+    (pts_to a p res);
+  res
